Low* wrapper for AESCTR + hints

vale/code/arch/x64/interop/GCTR_stdcalls.fst
@@ -10,14 +10,23 @@ open GCM_helpers
 open Workarounds
 open Arch.Types
 
+let length_aux3 (b:uint8_p) (n:nat) : Lemma
+  (requires B.length b = 16 * n)
+  (ensures DV.length (get_downview b) % 16 = 0) =
+    let db = get_downview b in
+    DV.length_eq db;
+    FStar.Math.Lemmas.cancel_mul_mod n 16
+
 inline_for_extraction
 val gctr128_bytes_stdcall':
   key:Ghost.erased (Seq.seq nat32) ->
   in_b:uint8_p ->
   num_bytes:uint64 ->
   out_b:uint8_p ->
+  inout_b: uint8_p ->
   keys_b:uint8_p ->
   ctr_b:uint8_p ->
+  num_blocks:uint64 ->
   Stack unit
   (requires fun h0 ->
      B.disjoint in_b out_b /\
@@ -26,16 +35,22 @@ val gctr128_bytes_stdcall':
      B.disjoint ctr_b in_b /\
      B.disjoint ctr_b out_b /\
      B.disjoint ctr_b keys_b /\
+     B.disjoint inout_b in_b /\ B.disjoint inout_b out_b /\
+     B.disjoint inout_b keys_b /\ B.disjoint inout_b ctr_b /\
 
      B.live h0 keys_b /\ B.live h0 in_b /\
      B.live h0 out_b /\ B.live h0 ctr_b /\
+     B.live h0 inout_b /\
 
-     B.length in_b = 16 * bytes_to_quad_size (UInt64.v num_bytes) /\
+     B.length in_b = 16 * UInt64.v num_blocks /\
      B.length out_b = B.length in_b /\
      B.length ctr_b = 16 /\
      B.length keys_b = AES_stdcalls.key_offset AES_128 /\
+     B.length inout_b = 16 /\
 
-     4096 * (UInt64.v num_bytes) < pow2_32 /\
+     4096 * (UInt64.v num_blocks) * 16 < pow2_32 /\
+     UInt64.v num_blocks * 128/8 <= UInt64.v num_bytes /\
+     UInt64.v num_bytes < UInt64.v num_blocks * 128/8 + 128/8 /\
 
      aesni_enabled /\
      is_aes_key_LE AES_128 (Ghost.reveal key) /\
@@ -43,11 +58,23 @@ val gctr128_bytes_stdcall':
        (seq_nat8_to_seq_uint8 (le_seq_quad32_to_bytes (key_to_round_keys_LE AES_128 (Ghost.reveal key)))))
    )
    (ensures fun h0 r h1 ->
-     B.modifies (B.loc_buffer out_b) h0 h1 /\
+     B.modifies (B.loc_union (B.loc_buffer out_b) (B.loc_buffer inout_b)) h0 h1 /\
 
      (let ctr = seq_uint8_to_seq_nat8 (B.as_seq h0 ctr_b) in
-      let plain = slice_work_around (seq_uint8_to_seq_nat8 (B.as_seq h0 in_b)) (UInt64.v num_bytes) in
-      let cipher = slice_work_around (seq_uint8_to_seq_nat8 (B.as_seq h1 out_b)) (UInt64.v num_bytes) in
+       let in_d = get_downview in_b in
+       length_aux3 in_b (UInt64.v num_blocks);
+       let in_u = UV.mk_buffer in_d Views.up_view128 in
+       let inout_d = get_downview inout_b in
+       length_aux3 inout_b 1;      
+       let inout_u = UV.mk_buffer inout_d Views.up_view128 in       
+       let out_d = get_downview out_b in
+       length_aux3 out_b (UInt64.v num_blocks);
+       let out_u = UV.mk_buffer out_d Views.up_view128 in
+
+      let plain_quads = Seq.append (UV.as_seq h0 in_u) (UV.as_seq h0 inout_u) in
+      let plain = slice_work_around (le_seq_quad32_to_bytes plain_quads) (UInt64.v num_bytes) in
+      let cipher_quads = Seq.append (UV.as_seq h1 out_u) (UV.as_seq h1 inout_u) in
+      let cipher = slice_work_around (le_seq_quad32_to_bytes cipher_quads) (UInt64.v num_bytes) in
       Seq.equal
         (gctr_encrypt_LE (le_bytes_to_quad32 ctr) (make_gctr_plain_LE plain) AES_128 (Ghost.reveal key))
         cipher
@@ -60,8 +87,10 @@ val gctr256_bytes_stdcall':
   in_b:uint8_p ->
   num_bytes:uint64 ->
   out_b:uint8_p ->
+  inout_b: uint8_p ->
   keys_b:uint8_p ->
   ctr_b:uint8_p ->
+  num_blocks:uint64 ->
   Stack unit
   (requires fun h0 ->
      B.disjoint in_b out_b /\
@@ -70,16 +99,22 @@ val gctr256_bytes_stdcall':
      B.disjoint ctr_b in_b /\
      B.disjoint ctr_b out_b /\
      B.disjoint ctr_b keys_b /\
+     B.disjoint inout_b in_b /\ B.disjoint inout_b out_b /\
+     B.disjoint inout_b keys_b /\ B.disjoint inout_b ctr_b /\
 
      B.live h0 keys_b /\ B.live h0 in_b /\
      B.live h0 out_b /\ B.live h0 ctr_b /\
+     B.live h0 inout_b /\
 
-     B.length in_b = 16 * bytes_to_quad_size (UInt64.v num_bytes) /\
+     B.length in_b = 16 * UInt64.v num_blocks /\
      B.length out_b = B.length in_b /\
      B.length ctr_b = 16 /\
      B.length keys_b = AES_stdcalls.key_offset AES_256 /\
+     B.length inout_b = 16 /\
 
-     4096 * (UInt64.v num_bytes) < pow2_32 /\
+     4096 * (UInt64.v num_blocks) * 16 < pow2_32 /\
+     UInt64.v num_blocks * 128/8 <= UInt64.v num_bytes /\
+     UInt64.v num_bytes < UInt64.v num_blocks * 128/8 + 128/8 /\
 
      aesni_enabled /\
      is_aes_key_LE AES_256 (Ghost.reveal key) /\
@@ -87,17 +122,30 @@ val gctr256_bytes_stdcall':
        (seq_nat8_to_seq_uint8 (le_seq_quad32_to_bytes (key_to_round_keys_LE AES_256 (Ghost.reveal key)))))
    )
    (ensures fun h0 r h1 ->
-     B.modifies (B.loc_buffer out_b) h0 h1 /\
+     B.modifies (B.loc_union (B.loc_buffer out_b) (B.loc_buffer inout_b)) h0 h1 /\
 
      (let ctr = seq_uint8_to_seq_nat8 (B.as_seq h0 ctr_b) in
-      let plain = slice_work_around (seq_uint8_to_seq_nat8 (B.as_seq h0 in_b)) (UInt64.v num_bytes) in
-      let cipher = slice_work_around (seq_uint8_to_seq_nat8 (B.as_seq h1 out_b)) (UInt64.v num_bytes) in
+
+       let in_d = get_downview in_b in
+       length_aux3 in_b (UInt64.v num_blocks);
+       let in_u = UV.mk_buffer in_d Views.up_view128 in
+       let inout_d = get_downview inout_b in
+       length_aux3 inout_b 1;      
+       let inout_u = UV.mk_buffer inout_d Views.up_view128 in       
+       let out_d = get_downview out_b in
+       length_aux3 out_b (UInt64.v num_blocks);
+       let out_u = UV.mk_buffer out_d Views.up_view128 in
+
+      let plain_quads = Seq.append (UV.as_seq h0 in_u) (UV.as_seq h0 inout_u) in
+      let plain = slice_work_around (le_seq_quad32_to_bytes plain_quads) (UInt64.v num_bytes) in
+      let cipher_quads = Seq.append (UV.as_seq h1 out_u) (UV.as_seq h1 inout_u) in
+      let cipher = slice_work_around (le_seq_quad32_to_bytes cipher_quads) (UInt64.v num_bytes) in
       Seq.equal
         (gctr_encrypt_LE (le_bytes_to_quad32 ctr) (make_gctr_plain_LE plain) AES_256 (Ghost.reveal key))
         cipher
       )
    )
-
+   
 let length_aux (b:uint8_p) : Lemma
   (requires B.length b = 176)
   (ensures DV.length (get_downview b) % 16 = 0) =
@@ -111,21 +159,21 @@ let length_aux2 (b:uint8_p) : Lemma
     DV.length_eq db
 
 #set-options "--z3rlimit 200 --max_fuel 0 --max_ifuel 0"
-
 inline_for_extraction
-let gctr128_bytes_stdcall' key in_b num_bytes out_b keys_b ctr_b =
+let gctr128_bytes_stdcall' key in_b num_bytes out_b inout_b keys_b ctr_b num_blocks =
   let h0 = get() in
-  FStar.Math.Lemmas.lemma_div_mod (bytes_to_quad_size (UInt64.v num_bytes)) 16;
 
   DV.length_eq (get_downview in_b);
   DV.length_eq (get_downview out_b);
   DV.length_eq (get_downview keys_b);
   DV.length_eq (get_downview ctr_b);
+  DV.length_eq (get_downview inout_b);
 
   as_vale_buffer_len #TUInt8 #TUInt128 in_b;
   as_vale_buffer_len #TUInt8 #TUInt128 out_b;
   as_vale_buffer_len #TUInt8 #TUInt128 keys_b;
   as_vale_buffer_len #TUInt8 #TUInt128 ctr_b;
+  as_vale_buffer_len #TUInt8 #TUInt128 inout_b;
 
   Classical.forall_intro (bounded_buffer_addrs TUInt8 TUInt128 h0 in_b);
   Classical.forall_intro (bounded_buffer_addrs TUInt8 TUInt128 h0 keys_b);
@@ -151,29 +199,32 @@ let gctr128_bytes_stdcall' key in_b num_bytes out_b keys_b ctr_b =
       }
 
   in lemma_uv_key ();
-  let x, _ = gctr128_bytes key in_b num_bytes out_b keys_b ctr_b () in
+  let x, _ = gctr128_bytes key in_b num_bytes out_b inout_b keys_b ctr_b num_blocks () in
 
   let h1 = get() in
 
-  lemma_seq_nat8_le_seq_quad32_to_bytes_uint32 in_b h1;
-  lemma_seq_nat8_le_seq_quad32_to_bytes_uint32 out_b h1; 
+  // lemma_seq_nat8_le_seq_quad32_to_bytes_uint32 in_b h1;
+  // lemma_seq_nat8_le_seq_quad32_to_bytes_uint32 inout_b h0;
+  // lemma_seq_nat8_le_seq_quad32_to_bytes_uint32 inout_b h1;
+  // lemma_seq_nat8_le_seq_quad32_to_bytes_uint32 out_b h1; 
   le_bytes_to_quad32_to_bytes (low_buffer_read TUInt8 TUInt128 h0 ctr_b 0);
   gcm_simplify2 ctr_b h0;
 
   ()
 
 inline_for_extraction
-let gctr256_bytes_stdcall' key in_b num_bytes out_b keys_b ctr_b =
+let gctr256_bytes_stdcall' key in_b num_bytes out_b inout_b keys_b ctr_b num_blocks =
   let h0 = get() in
-  FStar.Math.Lemmas.lemma_div_mod (bytes_to_quad_size (UInt64.v num_bytes)) 16;
 
   DV.length_eq (get_downview in_b);
   DV.length_eq (get_downview out_b);
+  DV.length_eq (get_downview inout_b);
   DV.length_eq (get_downview keys_b);
   DV.length_eq (get_downview ctr_b);
 
   as_vale_buffer_len #TUInt8 #TUInt128 in_b;
   as_vale_buffer_len #TUInt8 #TUInt128 out_b;
+  as_vale_buffer_len #TUInt8 #TUInt128 inout_b;
   as_vale_buffer_len #TUInt8 #TUInt128 keys_b;
   as_vale_buffer_len #TUInt8 #TUInt128 ctr_b;
 
@@ -201,16 +252,139 @@ let gctr256_bytes_stdcall' key in_b num_bytes out_b keys_b ctr_b =
       }
 
   in lemma_uv_key ();
-  let x, _ = gctr256_bytes key in_b num_bytes out_b keys_b ctr_b () in
+  let x, _ = gctr256_bytes key in_b num_bytes out_b inout_b keys_b ctr_b num_blocks () in
 
   let h1 = get() in
 
-  lemma_seq_nat8_le_seq_quad32_to_bytes_uint32 in_b h1;
-  lemma_seq_nat8_le_seq_quad32_to_bytes_uint32 out_b h1; 
+  // lemma_seq_nat8_le_seq_quad32_to_bytes_uint32 in_b h1;
+  // lemma_seq_nat8_le_seq_quad32_to_bytes_uint32 out_b h1; 
   le_bytes_to_quad32_to_bytes (low_buffer_read TUInt8 TUInt128 h0 ctr_b 0);
   gcm_simplify2 ctr_b h0;
 
   ()
+
+let length_aux4 (b:uint8_p) (n:nat) : Lemma
+  (requires B.length b = n * 16)
+  (ensures DV.length (get_downview b) % 16 = 0) =
+  DV.length_eq (get_downview b)
+
+let length_aux6 (b:uint8_p) : Lemma (B.length b = DV.length (get_downview b))
+  = DV.length_eq (get_downview b)
+
+let lemma_slice_uv_extra (b:uint8_p) (b_start:uint8_p) (b_extra:uint8_p) (h:HS.mem) : Lemma
+  (requires 
+    B.length b_start = B.length b / 16 * 16 /\
+    b_start == B.gsub b 0ul (UInt32.uint_to_t (B.length b_start)) /\ 
+    B.length b_extra = 16 /\
+    Seq.equal 
+      (B.as_seq h b)
+      (Seq.slice (Seq.append (B.as_seq h b_start) (B.as_seq h b_extra)) 0 (B.length b))
+    )
+  (ensures (
+    let b_start_d = get_downview b_start in
+    length_aux4 b_start (B.length b / 16);
+    let b_start_u = UV.mk_buffer b_start_d Views.up_view128 in
+    let b_extra_d = get_downview b_extra in
+    length_aux4 b_extra 1;
+    let b_extra_u = UV.mk_buffer b_extra_d Views.up_view128 in
+    let suv = Seq.append (UV.as_seq h b_start_u) (UV.as_seq h b_extra_u) in
+    let sf = slice_work_around (le_seq_quad32_to_bytes suv) (B.length b) in
+    Seq.equal sf (seq_uint8_to_seq_nat8 (B.as_seq h b))
+ ))
+ =
+ let b_start_d = get_downview b_start in
+ length_aux6 b_start;
+ let b_start_u = UV.mk_buffer b_start_d Views.up_view128 in
+ let b_extra_d = get_downview b_extra in
+ length_aux6 b_extra;
+ let b_extra_u = UV.mk_buffer b_extra_d Views.up_view128 in
+ let suv = Seq.append (UV.as_seq h b_start_u) (UV.as_seq h b_extra_u) in
+ let sf = slice_work_around (le_seq_quad32_to_bytes suv) (B.length b) in
+ let b_f = seq_uint8_to_seq_nat8 (B.as_seq h b) in
+ // if B.length b > B.length b_start then (
+   calc (==) {
+     sf;
+     (==) { DV.length_eq b_start_d; lemma_seq_nat8_le_seq_quad32_to_bytes_uint32 b_start h;
+          le_bytes_to_seq_quad32_to_bytes (UV.as_seq h b_start_u) }
+     slice_work_around (le_seq_quad32_to_bytes (Seq.append 
+       (le_bytes_to_seq_quad32 (seq_uint8_to_seq_nat8 (B.as_seq h b_start)))
+       (UV.as_seq h b_extra_u)))
+     (B.length b);
+     (==) { DV.length_eq b_extra_d; lemma_seq_nat8_le_seq_quad32_to_bytes_uint32 b_extra h;
+       le_bytes_to_seq_quad32_to_bytes (UV.as_seq h b_extra_u) }
+     slice_work_around (le_seq_quad32_to_bytes (Seq.append 
+       (le_bytes_to_seq_quad32 (seq_uint8_to_seq_nat8 (B.as_seq h b_start)))
+       (le_bytes_to_seq_quad32 (seq_uint8_to_seq_nat8 (B.as_seq h b_extra)))))
+     (B.length b);
+     (==) { append_distributes_le_seq_quad32_to_bytes
+        (le_bytes_to_seq_quad32 (seq_uint8_to_seq_nat8 (B.as_seq h b_start)))
+        (le_bytes_to_seq_quad32 (seq_uint8_to_seq_nat8 (B.as_seq h b_extra)))
+        }
+     slice_work_around (Seq.append
+       (le_seq_quad32_to_bytes (le_bytes_to_seq_quad32 (seq_uint8_to_seq_nat8 (B.as_seq h b_start))))
+       (le_seq_quad32_to_bytes (le_bytes_to_seq_quad32 (seq_uint8_to_seq_nat8 (B.as_seq h b_extra)))))
+     (B.length b);
+     (==) { le_seq_quad32_to_bytes_to_seq_quad32 (seq_uint8_to_seq_nat8 (B.as_seq h b_start));
+            le_seq_quad32_to_bytes_to_seq_quad32 (seq_uint8_to_seq_nat8 (B.as_seq h b_extra)) }
+     slice_work_around (Seq.append
+       (seq_uint8_to_seq_nat8 (B.as_seq h b_start))
+       (seq_uint8_to_seq_nat8 (B.as_seq h b_extra)))
+     (B.length b);
+     (==) { Seq.lemma_eq_intro b_f
+       (slice_work_around (Seq.append
+         (seq_uint8_to_seq_nat8 (B.as_seq h b_start))
+         (seq_uint8_to_seq_nat8 (B.as_seq h b_extra)))
+       (B.length b))
+     }
+     b_f;
+   }
+
+let lemma_slice_sub (b:uint8_p) (b_sub:uint8_p) (b_extra:uint8_p) (h:HS.mem) : Lemma
+  (requires B.length b_extra = 16 /\ B.length b_sub = B.length b / 16 * 16 /\
+    b_sub == B.gsub b 0ul (UInt32.uint_to_t (B.length b_sub)) /\
+    Seq.equal
+      (Seq.slice (B.as_seq h b) (B.length b_sub) (B.length b_sub + B.length b % 16))
+      (Seq.slice (B.as_seq h b_extra) 0 (B.length b % 16))
+  )
+  (ensures Seq.equal
+    (B.as_seq h b)
+    (Seq.slice (Seq.append (B.as_seq h b_sub) (B.as_seq h b_extra)) 0 (B.length b))
+  ) =
+  calc (==) {
+    Seq.slice (Seq.append (B.as_seq h b_sub) (B.as_seq h b_extra)) 0 (B.length b);
+    (==) { Seq.lemma_eq_intro
+     (Seq.slice (Seq.append (B.as_seq h b_sub) (B.as_seq h b_extra)) 0 (B.length b))
+     (Seq.append (B.as_seq h b_sub) (Seq.slice (B.as_seq h b_extra) 0 (B.length b % 16)))
+    }
+    Seq.append (B.as_seq h b_sub) (Seq.slice (B.as_seq h b_extra) 0 (B.length b % 16));
+    (==) { }
+    Seq.append 
+      (Seq.slice (B.as_seq h b) 0 (B.length b_sub))
+      (Seq.slice (B.as_seq h b_extra) 0 (B.length b % 16));      
+    (==) { }
+    Seq.append 
+      (Seq.slice (B.as_seq h b) 0 (B.length b_sub))
+      (Seq.slice (B.as_seq h b) (B.length b_sub) (B.length b));
+    (==) { Seq.lemma_eq_intro (B.as_seq h b)
+      (Seq.append 
+        (Seq.slice (B.as_seq h b) 0 (B.length b_sub))
+        (Seq.slice (B.as_seq h b) (B.length b_sub) (B.length b)))
+      }
+    B.as_seq h b;
+  }
+
+open BufferViewHelpers
+
+let lemma_identical_uv (b:uint8_p) (h0 h1:HS.mem) : Lemma
+  (requires B.length b % 16 = 0 /\ Seq.equal (B.as_seq h0 b) (B.as_seq h1 b))
+  (ensures (
+    let b_d = get_downview b in
+    length_aux3 b (B.length b / 16);
+    let b_u = UV.mk_buffer b_d Views.up_view128 in
+    Seq.equal (UV.as_seq h0 b_u) (UV.as_seq h1 b_u)))
+  = lemma_dv_equal Views.down_view8 b h0 h1;
+    length_aux3 b (B.length b / 16);
+    lemma_uv_equal Views.up_view128 (get_downview b) h0 h1
 
 
 open FStar.Integers
@@ -233,71 +407,110 @@ let bytes_to_quad_size_st (l:UInt32.t{4096 * UInt32.v l < pow2_32}) : Tot
 
 let gctr_bytes_stdcall128 key in_b num_bytes out_b keys_b ctr_b =
   push_frame();
+  let inout_b = B.alloca 0uy 16ul in
 
+  
   math_cast_aux num_bytes;
-  let num_bytes' = uint64_to_uint32 num_bytes in
+  let num_blocks = (uint64_to_uint32 num_bytes / 16ul) in
+  let num_bytes' = num_blocks * 16ul in
+  let in_b' = B.sub in_b 0ul num_bytes' in
+  let out_b' = B.sub out_b 0ul num_bytes' in
 
-  let in_extlength = bytes_to_quad_size_st num_bytes' in
-
-  // Allocate buffers that 'extend' initial buffers
-  // Dirty hack: The length could be 0 and we cannot allocate a buffer of size 0.
-  let in_extra = B.alloca 0uy (in_extlength + 1ul) in
-  let out_extra = B.alloca 0uy (in_extlength + 1ul) in
-
-  let in_extra = B.sub in_extra 0ul in_extlength in
-  let out_extra = B.sub out_extra 0ul in_extlength in
-
-  // Copy the initial contents in these buffers
-  B.blit in_b 0ul in_extra 0ul num_bytes';
+  B.blit in_b num_bytes' inout_b 0ul (uint64_to_uint32 num_bytes % 16ul);
 
   let h0 = get() in
-  assert (Seq.equal
-    (slice_work_around (seq_uint8_to_seq_nat8 (B.as_seq h0 in_extra)) (UInt64.v num_bytes))
-    (seq_uint8_to_seq_nat8 (B.as_seq h0 in_b)));
 
-  let _ = gctr128_bytes_stdcall' key in_extra num_bytes out_extra keys_b ctr_b in
+  let _ = gctr128_bytes_stdcall' key in_b' num_bytes out_b' inout_b keys_b ctr_b (uint32_to_uint64 num_blocks) in
 
-  B.blit out_extra 0ul out_b 0ul num_bytes';
+  let h_post = get() in
+
+  assert (let ctr = seq_uint8_to_seq_nat8 (B.as_seq h0 ctr_b) in
+
+       let in_d = get_downview in_b' in
+       length_aux3 in_b' (UInt64.v (uint32_to_uint64 num_blocks));
+       let in_u = UV.mk_buffer in_d Views.up_view128 in
+       let inout_d = get_downview inout_b in
+       length_aux3 inout_b 1;      
+       let inout_u = UV.mk_buffer inout_d Views.up_view128 in       
+       let out_d = get_downview out_b' in
+       length_aux3 out_b' (UInt64.v (uint32_to_uint64 num_blocks));
+       let out_u = UV.mk_buffer out_d Views.up_view128 in
+
+      let plain_quads = Seq.append (UV.as_seq h0 in_u) (UV.as_seq h0 inout_u) in
+      let plain = slice_work_around (le_seq_quad32_to_bytes plain_quads) (UInt64.v num_bytes) in
+      let cipher_quads = Seq.append (UV.as_seq h_post out_u) (UV.as_seq h_post inout_u) in
+      let cipher = slice_work_around (le_seq_quad32_to_bytes cipher_quads) (UInt64.v num_bytes) in
+      Seq.equal
+        (gctr_encrypt_LE (le_bytes_to_quad32 ctr) (make_gctr_plain_LE plain) AES_128 (Ghost.reveal key))
+        cipher);
+
+
+  B.blit inout_b 0ul out_b num_bytes' (uint64_to_uint32 num_bytes % 16ul);
 
   let h1 = get() in
-  assert (Seq.equal
-    (slice_work_around (seq_uint8_to_seq_nat8 (B.as_seq h1 out_extra)) (UInt64.v num_bytes))
-    (seq_uint8_to_seq_nat8 (B.as_seq h1 out_b)));
+
+  lemma_identical_uv out_b' h_post h1;
+  lemma_identical_uv inout_b h_post h1;
+  
+  lemma_slice_sub out_b out_b' inout_b h1;
+  lemma_slice_uv_extra out_b out_b' inout_b h1;
+
+  lemma_slice_sub in_b in_b' inout_b h0;
+  lemma_slice_uv_extra in_b in_b' inout_b h0;
 
   pop_frame()
 
-
 let gctr_bytes_stdcall256 key in_b num_bytes out_b keys_b ctr_b =
   push_frame();
+  let inout_b = B.alloca 0uy 16ul in
 
+  
   math_cast_aux num_bytes;
-  let num_bytes' = uint64_to_uint32 num_bytes in
+  let num_blocks = (uint64_to_uint32 num_bytes / 16ul) in
+  let num_bytes' = num_blocks * 16ul in
+  let in_b' = B.sub in_b 0ul num_bytes' in
+  let out_b' = B.sub out_b 0ul num_bytes' in
 
-  let in_extlength = bytes_to_quad_size_st num_bytes' in
-
-  // Allocate buffers that 'extend' initial buffers
-  // Dirty hack: The length could be 0 and we cannot allocate a buffer of size 0.
-  let in_extra = B.alloca 0uy (in_extlength + 1ul) in
-  let out_extra = B.alloca 0uy (in_extlength + 1ul) in
-
-  let in_extra = B.sub in_extra 0ul in_extlength in
-  let out_extra = B.sub out_extra 0ul in_extlength in
-
-  // Copy the initial contents in these buffers
-  B.blit in_b 0ul in_extra 0ul num_bytes';
+  B.blit in_b num_bytes' inout_b 0ul (uint64_to_uint32 num_bytes % 16ul);
 
   let h0 = get() in
-  assert (Seq.equal
-    (slice_work_around (seq_uint8_to_seq_nat8 (B.as_seq h0 in_extra)) (UInt64.v num_bytes))
-    (seq_uint8_to_seq_nat8 (B.as_seq h0 in_b)));
 
-  let _ = gctr256_bytes_stdcall' key in_extra num_bytes out_extra keys_b ctr_b in
+  let _ = gctr256_bytes_stdcall' key in_b' num_bytes out_b' inout_b keys_b ctr_b (uint32_to_uint64 num_blocks) in
 
-  B.blit out_extra 0ul out_b 0ul num_bytes';
+  let h_post = get() in
+
+  assert (let ctr = seq_uint8_to_seq_nat8 (B.as_seq h0 ctr_b) in
+
+       let in_d = get_downview in_b' in
+       length_aux3 in_b' (UInt64.v (uint32_to_uint64 num_blocks));
+       let in_u = UV.mk_buffer in_d Views.up_view128 in
+       let inout_d = get_downview inout_b in
+       length_aux3 inout_b 1;      
+       let inout_u = UV.mk_buffer inout_d Views.up_view128 in       
+       let out_d = get_downview out_b' in
+       length_aux3 out_b' (UInt64.v (uint32_to_uint64 num_blocks));
+       let out_u = UV.mk_buffer out_d Views.up_view128 in
+
+      let plain_quads = Seq.append (UV.as_seq h0 in_u) (UV.as_seq h0 inout_u) in
+      let plain = slice_work_around (le_seq_quad32_to_bytes plain_quads) (UInt64.v num_bytes) in
+      let cipher_quads = Seq.append (UV.as_seq h_post out_u) (UV.as_seq h_post inout_u) in
+      let cipher = slice_work_around (le_seq_quad32_to_bytes cipher_quads) (UInt64.v num_bytes) in
+      Seq.equal
+        (gctr_encrypt_LE (le_bytes_to_quad32 ctr) (make_gctr_plain_LE plain) AES_256 (Ghost.reveal key))
+        cipher);
+
+
+  B.blit inout_b 0ul out_b num_bytes' (uint64_to_uint32 num_bytes % 16ul);
 
   let h1 = get() in
-  assert (Seq.equal
-    (slice_work_around (seq_uint8_to_seq_nat8 (B.as_seq h1 out_extra)) (UInt64.v num_bytes))
-    (seq_uint8_to_seq_nat8 (B.as_seq h1 out_b)));
+
+  lemma_identical_uv out_b' h_post h1;
+  lemma_identical_uv inout_b h_post h1;
+  
+  lemma_slice_sub out_b out_b' inout_b h1;
+  lemma_slice_uv_extra out_b out_b' inout_b h1;
+
+  lemma_slice_sub in_b in_b' inout_b h0;
+  lemma_slice_uv_extra in_b in_b' inout_b h0;
 
   pop_frame()
